Merge pull request #678 from MetaCoq/eenvmap-in-optimize-prop-discr
Use an EEnvMap in OptimizePropDiscr for more efficient lookups

(cherry picked from commit 4ee54ae46c07d0c3bc8d8e9778869a2ecfcf31cd)

erasure/theories/EOptimizePropDiscr.v
@@ -8,7 +8,7 @@ From MetaCoq.PCUIC Require Import PCUICAst PCUICAstUtils
 From MetaCoq.SafeChecker Require Import PCUICWfEnvImpl.
 From MetaCoq.Erasure Require Import EAst EAstUtils EDeps EExtends
     ELiftSubst ECSubst EGlobalEnv EWellformed EWcbvEval Extract Prelim
-    ErasureFunction EArities EProgram.
+    EEnvMap EArities EProgram.
 
 Local Open Scope string_scope.
 Set Asymmetric Patterns.
@@ -28,7 +28,7 @@ Ltac introdep := let H := fresh in intros H; depelim H.
 Hint Constructors eval : core.
 
 Section optimize.
-  Context (Σ : global_context).
+  Context (Σ : GlobalContextMap.t).
 
   Fixpoint optimize (t : term) : term :=
     match t with
@@ -39,7 +39,7 @@ Section optimize.
     | tLetIn na b b' => tLetIn na (optimize b) (optimize b')
     | tCase ind c brs =>
       let brs' := List.map (on_snd optimize) brs in
-      match EGlobalEnv.inductive_isprop_and_pars Σ (fst ind) with
+      match GlobalContextMap.inductive_isprop_and_pars Σ (fst ind) with
       | Some (true, npars) =>
         match brs' with
         | [(a, b)] => ECSubst.substl (repeat tBox #|a|) b
@@ -48,7 +48,7 @@ Section optimize.
       | _ => tCase ind (optimize c) brs'
       end
     | tProj p c =>
-      match EGlobalEnv.inductive_isprop_and_pars Σ p.1.1 with 
+      match GlobalContextMap.inductive_isprop_and_pars Σ p.1.1 with 
       | Some (true, _) => tBox
       | _ => tProj p (optimize c)
       end
@@ -107,7 +107,8 @@ Section optimize.
     rewrite -> ?map_map_compose, ?compose_on_snd, ?compose_map_def, ?map_length;
     unfold test_def in *;
     simpl closed in *; try solve [simpl subst; simpl closed; f_equal; auto; rtoProp; solve_all]; try easy.
-    - move/andP: H => [] clt cll. destruct EGlobalEnv.inductive_isprop_and_pars as [[[|] _]|] => /= //.
+    - move/andP: H => [] clt cll. 
+      destruct GlobalContextMap.inductive_isprop_and_pars as [[[|] _]|] => /= //.
       destruct l as [|[br n] [|l']] eqn:eql; simpl.
       rewrite IHt //.
       depelim X. cbn in *.
@@ -120,7 +121,7 @@ Section optimize.
       depelim cll. depelim cll. solve_all.
       rtoProp; solve_all. solve_all.
       rtoProp; solve_all. solve_all.
-    - destruct EGlobalEnv.inductive_isprop_and_pars as [[[|] _]|]; cbn; auto.
+    - destruct GlobalContextMap.inductive_isprop_and_pars as [[[|] _]|]; cbn; auto.
   Qed.
  
   Lemma subst_csubst_comm l t k b : 
@@ -159,13 +160,6 @@ Section optimize.
     apply subst_csubst_comm => //.
   Qed.
 
-  (* Lemma is_box_fix_csubst a m n k : is_box_fix m n = is_box_fix (map (map_def (csubst a (#|m| + k))) m) n.
-  Proof.
-    unfold is_box_fix. rewrite nth_error_map. destruct nth_error as [[]|] => /=.
-     *)
-  Import EEtaExpanded.
-  Ltac solve_discr' := try solve_discr; repeat solve_discr_args; try congruence.
-
   Lemma optimize_csubst a k b : 
     closed a ->
     optimize (ECSubst.csubst a k b) = ECSubst.csubst (optimize a) k (optimize b).
@@ -176,9 +170,9 @@ Section optimize.
     unfold test_def in *;
     simpl closed in *; try solve [simpl subst; simpl closed; f_equal; auto; rtoProp; solve_all]; try easy.
     - destruct (k ?= n)%nat; auto.
-    - unfold on_snd; cbn.
-      destruct EGlobalEnv.inductive_isprop_and_pars as [[[|] _]|] => /= //.
+    - destruct GlobalContextMap.inductive_isprop_and_pars as [[[|] _]|] => /= //.
       destruct l as [|[br n] [|l']] eqn:eql; simpl.
+      all:unfold on_snd; cbn.
       * f_equal; auto.
       * depelim X. simpl in *.
         rewrite e //.
@@ -188,13 +182,14 @@ Section optimize.
         solve_all. eapply All_repeat => //.
         now eapply closed_optimize.
       * depelim X. depelim X.
-        f_equal; eauto. f_equal; eauto.
+        f_equal; eauto.
+        unfold on_snd; cbn. f_equal; eauto.
         f_equal; eauto.
         f_equal; eauto. f_equal; eauto.
         rewrite map_map_compose; solve_all.
       * rewrite ?map_map_compose; f_equal; eauto; solve_all.
       * rewrite ?map_map_compose; f_equal; eauto; solve_all.
-    - destruct EGlobalEnv.inductive_isprop_and_pars as [[[|] _]|]=> //;
+    - destruct GlobalContextMap.inductive_isprop_and_pars as [[[|] _]|]=> //;
       now rewrite IHb.
   Qed.
 
@@ -311,34 +306,6 @@ Proof.
   eexists; econstructor; eauto.
 Qed.
 
-Import ErasureCorrectness.
-
-Lemma erasable_tBox_value (wfl := Ee.default_wcbv_flags) (Σ : global_env_ext) (wfΣ : wf_ext Σ) t T v :
-  forall wt : Σ ;;; [] |- t : T,
-  Σ |-p t ▷ v -> erases Σ [] v tBox -> ∥ isErasable Σ [] t ∥.
-Proof.
-  intros.
-  depind H.
-  eapply Is_type_eval_inv; eauto. eexists; eauto.
-Qed.
-
-Lemma erase_eval_to_box (wfl := Ee.default_wcbv_flags) {Σ : wf_env} {univs wfext t v Σ' t' deps} :
-  let Σext := make_wf_env_ext Σ univs wfext in
-  forall wt : ∀ Σ0 : global_env_ext, abstract_env_rel' Σext Σ0 →  welltyped Σ0 [] t,
-  erase Σext [] t wt = t' ->
-  KernameSet.subset (term_global_deps t') deps ->
-  erase_global deps Σ = Σ' ->
-  PCUICWcbvEval.eval Σ t v ->
-  @Ee.eval Ee.default_wcbv_flags Σ' t' tBox -> ∥ isErasable Σext [] t ∥.
-Proof.
-  intros Σext wt.
-  intros.
-  destruct (erase_correct Σ univs wfext _ _ _ _ _ wt H H0 H1 X) as [ev [eg [eg']]].
-  pose proof (Ee.eval_deterministic H2 eg'). subst.
-  destruct wfext. destruct (wt _ eq_refl) as [T wt'].
-  eapply erasable_tBox_value; eauto.
-Qed.
-
 Definition optimize_constant_decl Σ cb := 
   {| cst_body := option_map (optimize Σ) cb.(cst_body) |}.
   
@@ -348,10 +315,17 @@ Definition optimize_decl Σ d :=
   | InductiveDecl idecl => d
   end.
 
-Fixpoint optimize_env (Σ : EAst.global_declarations) := 
+Definition optimize_env Σ := 
+  map (on_snd (optimize_decl Σ)) Σ.(GlobalContextMap.global_decls).
+  
+Import EnvMap.
+
+Program Fixpoint optimize_env' Σ : EnvMap.fresh_globals Σ -> global_context :=
   match Σ with
-  | [] => []
-  | d :: Σ => on_snd (optimize_decl Σ) d :: optimize_env Σ
+  | [] => fun _ => []
+  | hd :: tl => fun HΣ =>
+    let Σg := GlobalContextMap.make tl (fresh_globals_cons_inv HΣ) in 
+    on_snd (optimize_decl Σg) hd :: optimize_env' tl (fresh_globals_cons_inv HΣ) 
   end.
 
 Import EGlobalEnv EExtends.
@@ -382,28 +356,31 @@ Proof.
   destruct nth_error => //.
 Qed.
 
-Lemma wellformed_optimize_extends {wfl: EEnvFlags} Σ t : 
+Lemma wellformed_optimize_extends {wfl: EEnvFlags} {Σ : GlobalContextMap.t} t : 
   forall n, EWellformed.wellformed Σ n t ->
-  forall Σ', extends Σ Σ' -> wf_glob Σ' ->
+  forall {Σ' : GlobalContextMap.t}, extends Σ Σ' -> wf_glob Σ' ->
   optimize Σ t = optimize Σ' t.
 Proof.
-  induction t using EInduction.term_forall_list_ind; cbn -[lookup_constant lookup_inductive]; intros => //.
+  induction t using EInduction.term_forall_list_ind; cbn -[lookup_constant lookup_inductive
+    GlobalContextMap.inductive_isprop_and_pars]; intros => //.
   all:rtoProp; intuition auto.  
   all:f_equal; eauto; solve_all.
-  - assert (map (on_snd (optimize Σ)) l = map (on_snd (optimize Σ')) l) as -> by solve_all.
+  - rewrite !GlobalContextMap.inductive_isprop_and_pars_spec.
+    assert (map (on_snd (optimize Σ)) l = map (on_snd (optimize Σ')) l) as -> by solve_all.
     rewrite (extends_inductive_isprop_and_pars H0 H1 H2).
     destruct inductive_isprop_and_pars as [[[]]|].
     destruct map => //. f_equal; eauto.
     destruct l0 => //. destruct p0 => //. f_equal; eauto.
     all:f_equal; eauto; solve_all.
-  - rewrite (extends_inductive_isprop_and_pars H0 H1 H3).
+  - rewrite !GlobalContextMap.inductive_isprop_and_pars_spec.
+    rewrite (extends_inductive_isprop_and_pars H0 H1 H3).
     destruct inductive_isprop_and_pars as [[[]]|] => //.
     all:f_equal; eauto.
 Qed.
 
-Lemma wellformed_optimize_decl_extends {wfl: EEnvFlags} Σ t : 
+Lemma wellformed_optimize_decl_extends {wfl: EEnvFlags} {Σ : GlobalContextMap.t} t : 
   wf_global_decl Σ t ->
-  forall Σ', extends Σ Σ' -> wf_glob Σ' ->
+  forall {Σ' : GlobalContextMap.t}, extends Σ Σ' -> wf_glob Σ' ->
   optimize_decl Σ t = optimize_decl Σ' t.
 Proof.
   destruct t => /= //.
@@ -411,51 +388,81 @@ Proof.
   destruct (cst_body c) => /= //. f_equal.
   now eapply wellformed_optimize_extends.
 Qed.
-  
 
-Lemma lookup_env_optimize_env_Some {efl : EEnvFlags} Σ kn d : 
+Lemma lookup_env_optimize_env_Some {efl : EEnvFlags} {Σ : GlobalContextMap.t} kn d : 
   wf_glob Σ ->
-  lookup_env Σ kn = Some d ->
-  ∑ Σ', extends Σ' Σ × wf_global_decl Σ' d × (lookup_env (optimize_env Σ) kn) = Some (optimize_decl Σ' d).
+  GlobalContextMap.lookup_env Σ kn = Some d ->
+  ∑ Σ' : GlobalContextMap.t, 
+    [× extends Σ' Σ, wf_global_decl Σ' d &
+      lookup_env (optimize_env Σ) kn = Some (optimize_decl Σ' d)].
 Proof.
-  induction Σ; simpl; auto => //.
-  intros wf.
+  rewrite GlobalContextMap.lookup_env_spec.
+  destruct Σ as [Σ map repr wf].
+  induction Σ in map, repr, wf |- *; simpl; auto => //.
+  intros wfg.
   case: eqb_specT => //.
-  - intros ->. cbn. intros [= <-]. exists Σ. split. now eexists [_]. split => //.
-    now depelim wf.
-  - intros _. forward IHΣ. now depelim wf.
-    intros hl. specialize (IHΣ hl) as [Σ' [[Σ'' ext] eq]].
-    subst Σ. exists Σ'. split => //. now exists (a :: Σ'').
+  - intros ->. cbn. intros [= <-].
+    exists (GlobalContextMap.make Σ (fresh_globals_cons_inv wf)). split.
+    now eexists [_].
+    cbn. now depelim wfg.
+    f_equal. symmetry. eapply wellformed_optimize_decl_extends. cbn. now depelim wfg.
+    cbn. now exists [a]. now cbn.
+  - intros _. 
+    set (Σ' := GlobalContextMap.make Σ (fresh_globals_cons_inv wf)).
+    specialize (IHΣ (GlobalContextMap.map Σ') (GlobalContextMap.repr Σ') (GlobalContextMap.wf Σ')).
+    cbn in IHΣ. forward IHΣ. now depelim wfg.
+    intros hl. specialize (IHΣ hl) as [Σ'' [ext wfgd hl']].
+    exists Σ''. split => //.
+    * destruct ext as [? ->].
+      now exists (a :: x).
+    * rewrite -hl'. f_equal.
+      clear -wfg.
+      eapply map_ext_in => kn hin. unfold on_snd. f_equal.
+      symmetry. eapply wellformed_optimize_decl_extends => //. cbn.
+      eapply lookup_env_In in hin. 2:now depelim wfg.
+      depelim wfg. eapply lookup_env_wellformed; tea.
+      cbn. now exists [a].
 Qed.
 
-Lemma lookup_env_optimize_env_None {efl : EEnvFlags} Σ kn : 
-  lookup_env Σ kn = None ->
+Lemma lookup_env_map_snd Σ f kn : lookup_env (List.map (on_snd f) Σ) kn = option_map f (lookup_env Σ kn).
+Proof.
+  induction Σ; cbn; auto.
+  case: eqb_spec => //.
+Qed.
+
+Lemma lookup_env_optimize_env_None {efl : EEnvFlags} {Σ : GlobalContextMap.t} kn : 
+  GlobalContextMap.lookup_env Σ kn = None ->
   lookup_env (optimize_env Σ) kn = None.
 Proof.
-  induction Σ; simpl; auto => //.
-  case: eqb_specT => //.
+  rewrite GlobalContextMap.lookup_env_spec.
+  destruct Σ as [Σ map repr wf].
+  cbn. intros hl. rewrite lookup_env_map_snd hl //.
 Qed.
 
-Lemma lookup_env_optimize {efl : EEnvFlags} Σ kn : 
+Lemma lookup_env_optimize {efl : EEnvFlags} {Σ : GlobalContextMap.t} kn : 
   wf_glob Σ ->
   lookup_env (optimize_env Σ) kn = option_map (optimize_decl Σ) (lookup_env Σ kn).
 Proof.
   intros wf.
-  destruct (lookup_env Σ kn) eqn:hl.
-  - eapply lookup_env_optimize_env_Some in hl as [Σ' [ext [wf' hl']]] => /=.
+  rewrite -GlobalContextMap.lookup_env_spec.
+  destruct (GlobalContextMap.lookup_env Σ kn) eqn:hl.
+  - eapply lookup_env_optimize_env_Some in hl as [Σ' [ext wf' hl']] => /=.
     rewrite hl'. f_equal.
     eapply wellformed_optimize_decl_extends; eauto. auto.
     
   - cbn. now eapply lookup_env_optimize_env_None in hl. 
 Qed.
 
-Lemma is_propositional_optimize {efl : EEnvFlags} Σ ind : 
+Lemma is_propositional_optimize {efl : EEnvFlags} {Σ : GlobalContextMap.t} ind : 
   wf_glob Σ ->
   inductive_isprop_and_pars Σ ind = inductive_isprop_and_pars (optimize_env Σ) ind.
 Proof.
   rewrite /inductive_isprop_and_pars => wf.
-  rewrite (lookup_env_optimize Σ (inductive_mind ind) wf).  
-  case: lookup_env => [[decl|]|] => //.
+  rewrite /lookup_inductive /lookup_minductive.
+  rewrite (lookup_env_optimize (inductive_mind ind) wf).
+  rewrite /GlobalContextMap.inductive_isprop_and_pars /GlobalContextMap.lookup_inductive
+    /GlobalContextMap.lookup_minductive.  
+  destruct lookup_env as [[decl|]|] => //.
 Qed.
 
 Lemma closed_iota_red pars c args brs br :
@@ -481,7 +488,7 @@ Proof.
   - rewrite mkApps_app /=. now destruct l => /= //; rewrite andb_false_r.
 Qed.
 
-Lemma optimize_correct {efl : EEnvFlags} {fl} Σ t v :
+Lemma optimize_correct {efl : EEnvFlags} {fl} {Σ : GlobalContextMap.t} t v :
   wf_glob Σ ->
   closed_env Σ ->
   @Ee.eval fl Σ t v ->
@@ -508,8 +515,9 @@ Proof.
     have := (eval_closed _ clΣ _ _ cld ev1); rewrite closedn_mkApps => /andP[] _ clargs.
     rewrite optimize_iota_red in IHev2.
     eapply eval_closed in ev1 => //.
-    destruct EGlobalEnv.inductive_isprop_and_pars as [[]|]eqn:isp => //. noconf e.
-    eapply Ee.eval_iota; eauto.
+    rewrite GlobalContextMap.inductive_isprop_and_pars_spec.
+    destruct inductive_isprop_and_pars as [[]|]eqn:isp => //. noconf e.
+    eapply eval_iota; eauto.
     now rewrite -is_propositional_optimize.
     rewrite nth_error_map e0 //. now len.
     eapply IHev2.
@@ -517,7 +525,9 @@ Proof.
     eapply nth_error_forallb in clbrs; tea. cbn in clbrs.
     now rewrite Nat.add_0_r in clbrs.
   
-  - move/andP => [] cld clbrs. rewrite e e0 /=.
+  - move/andP => [] cld clbrs.
+    rewrite GlobalContextMap.inductive_isprop_and_pars_spec.
+    rewrite e e0 /=.
     subst brs. cbn in clbrs. rewrite Nat.add_0_r andb_true_r in clbrs.
     rewrite optimize_substl in IHev2. 
     eapply All_forallb, All_repeat => //.
@@ -571,6 +581,7 @@ Proof.
     { rewrite clargs clbrs !andb_true_r.
       eapply closed_cunfold_cofix; tea. }
     rewrite -> optimize_mkApps in IHev1, IHev2. simpl.
+    rewrite GlobalContextMap.inductive_isprop_and_pars_spec in IHev2 |- *.
     destruct EGlobalEnv.inductive_isprop_and_pars as [[[] pars]|] eqn:isp => //.
     destruct brs as [|[a b] []]; simpl in *; auto.
     simpl in IHev1.
@@ -589,6 +600,7 @@ Proof.
     move: (eval_closed _ clΣ _ _ cd ev1).
     rewrite closedn_mkApps; move/andP => [] clfix clargs. forward IHev2.
     { rewrite closedn_mkApps clargs andb_true_r. eapply closed_cunfold_cofix; tea. }
+    rewrite GlobalContextMap.inductive_isprop_and_pars_spec in IHev2 |- *.
     destruct EGlobalEnv.inductive_isprop_and_pars as [[[] pars]|] eqn:isp; auto.
     rewrite -> optimize_mkApps in IHev1, IHev2. simpl in *.
     econstructor; eauto.
@@ -598,7 +610,8 @@ Proof.
     apply optimize_cunfold_cofix; tea. eapply closed_cofix_subst; tea.
   
   - rewrite /declared_constant in isdecl.
-    move: (lookup_env_optimize Σ c wfΣ); rewrite isdecl /= //.
+    move: (lookup_env_optimize c wfΣ).
+    rewrite isdecl /= //.
     intros hl.
     econstructor; tea. cbn. rewrite e //.
     apply IHev.
@@ -608,6 +621,7 @@ Proof.
   - move=> cld.
     eapply eval_closed in ev1; tea.
     move: ev1; rewrite closedn_mkApps /= => clargs.
+    rewrite GlobalContextMap.inductive_isprop_and_pars_spec.
     destruct EGlobalEnv.inductive_isprop_and_pars as [[[] pars']|] eqn:isp => //.
     rewrite optimize_mkApps in IHev1.
     rewrite optimize_nth in IHev2.
@@ -619,7 +633,8 @@ Proof.
     destruct nth_error eqn:hnth => //.
     eapply nth_error_forallb in hnth; tea.
 
-  - now rewrite e.
+  - rewrite GlobalContextMap.inductive_isprop_and_pars_spec.
+    now rewrite e.
 
   - move/andP => [] clf cla.
     specialize (IHev1 clf). specialize (IHev2 cla).
@@ -661,13 +676,14 @@ Proof. destruct t => //. Qed.
 Lemma isBox_optimize Σ t : isBox t -> isBox (optimize Σ t).
 Proof. destruct t => //. Qed.
 
-Lemma optimize_expanded Σ t : expanded Σ t -> expanded Σ (optimize Σ t).
+Lemma optimize_expanded {Σ : GlobalContextMap.t} t : expanded Σ t -> expanded Σ (optimize Σ t).
 Proof.
   induction 1 using expanded_ind.
   all:try solve[constructor; eauto; solve_all].
   all:rewrite ?optimize_mkApps.
   - eapply expanded_mkApps_expanded => //. solve_all.
-  - cbn.
+  - cbn -[GlobalContextMap.inductive_isprop_and_pars].
+    rewrite GlobalContextMap.inductive_isprop_and_pars_spec.
     destruct inductive_isprop_and_pars as [[[|] _]|] => /= //.
     2-3:constructor; eauto; solve_all.
     destruct branches eqn:heq.
@@ -681,7 +697,8 @@ Proof.
     constructor; eauto; solve_all.
     depelim H1. depelim H1. do 2 (constructor; intuition auto).
     solve_all.
-  - cbn.
+  - cbn -[GlobalContextMap.inductive_isprop_and_pars].
+    rewrite GlobalContextMap.inductive_isprop_and_pars_spec.
     destruct inductive_isprop_and_pars as [[[|] _]|] => /= //.
     constructor. all:constructor; auto.
   - cbn. eapply expanded_tFix. solve_all.
@@ -690,7 +707,7 @@ Proof.
     now len. solve_all.
 Qed.
 
-Lemma optimize_expanded_irrel {efl : EEnvFlags} Σ t : wf_glob Σ -> expanded Σ t -> expanded (optimize_env Σ) t.
+Lemma optimize_expanded_irrel {efl : EEnvFlags} {Σ : GlobalContextMap.t} t : wf_glob Σ -> expanded Σ t -> expanded (optimize_env Σ) t.
 Proof.
   intros wf; induction 1 using expanded_ind.
   all:try solve[constructor; eauto; solve_all].
@@ -700,39 +717,87 @@ Proof.
   red in H. rewrite lookup_env_optimize // /= H //. 1-2:eauto. auto. solve_all. 
 Qed.
 
-Lemma optimize_expanded_decl Σ t : expanded_decl Σ t -> expanded_decl Σ (optimize_decl Σ t).
+Lemma optimize_expanded_decl {Σ : GlobalContextMap.t} t : expanded_decl Σ t -> expanded_decl Σ (optimize_decl Σ t).
 Proof.
   destruct t as [[[]]|] => /= //.
   unfold expanded_constant_decl => /=.
   apply optimize_expanded.
 Qed.
 
-Lemma optimize_expanded_decl_irrel {efl : EEnvFlags} Σ t : wf_glob Σ -> expanded_decl Σ t -> expanded_decl (optimize_env Σ) t.
+Lemma optimize_expanded_decl_irrel {efl : EEnvFlags} {Σ : GlobalContextMap.t} t : wf_glob Σ -> expanded_decl Σ t -> expanded_decl (optimize_env Σ) t.
 Proof.
   destruct t as [[[]]|] => /= //.
   unfold expanded_constant_decl => /=.
   apply optimize_expanded_irrel.
 Qed.
 
-Lemma optimize_env_expanded {efl : EEnvFlags} Σ :
-  wf_glob Σ -> expanded_global_env Σ -> expanded_global_env (optimize_env Σ).
+Lemma optimize_env_extends' {efl : EEnvFlags} {Σ Σ' : GlobalContextMap.t} : 
+  extends Σ Σ' ->
+  wf_glob Σ' -> 
+  List.map (on_snd (optimize_decl Σ)) Σ.(GlobalContextMap.global_decls) =
+  List.map (on_snd (optimize_decl Σ')) Σ.(GlobalContextMap.global_decls).
 Proof.
-  unfold expanded_global_env.
-  intros wf. induction 1; cbn; constructor; auto.
-  now depelim wf. cbn. 
-  eapply optimize_expanded_decl in H0.
-  depelim wf; now eapply optimize_expanded_decl_irrel.
+  intros ext.
+  destruct Σ as [Σ map repr wf]; cbn in *.
+  move=> wfΣ.
+  assert (extends Σ Σ); auto. now exists [].
+  assert (wf_glob Σ).
+  { eapply extends_wf_glob. exact ext. tea. }
+  revert H H0.
+  generalize Σ at 1 3 5 6. intros Σ''.
+  induction Σ'' => //. cbn.
+  intros hin wfg. depelim wfg.
+  f_equal.
+  2:{ eapply IHΣ'' => //. destruct hin. exists (x ++ [(kn, d)]). rewrite -app_assoc /= //. }
+  unfold on_snd. cbn. f_equal.
+  eapply wellformed_optimize_decl_extends => //. cbn.
+  eapply extends_wf_global_decl. 3:tea.
+  eapply extends_wf_glob; tea.
+  destruct hin. exists (x ++ [(kn, d)]). rewrite -app_assoc /= //.
 Qed.
 
-Lemma optimize_wellformed {efl : EEnvFlags} Σ n t :
+Lemma optimize_env_eq {efl : EEnvFlags} (Σ : GlobalContextMap.t) : wf_glob Σ -> optimize_env Σ = optimize_env' Σ.(GlobalContextMap.global_decls) Σ.(GlobalContextMap.wf).
+Proof.
+  intros wf.
+  unfold optimize_env.
+  destruct Σ; cbn. cbn in wf.
+  induction global_decls in map, repr, wf0, wf |- * => //.
+  cbn. f_equal.
+  destruct a as [kn d]; unfold on_snd; cbn. f_equal. symmetry.
+  eapply wellformed_optimize_decl_extends => //. cbn. now depelim wf. cbn. now exists [(kn, d)]. cbn.
+  set (Σg' := GlobalContextMap.make global_decls (fresh_globals_cons_inv wf0)).
+  erewrite <- (IHglobal_decls (GlobalContextMap.map Σg') (GlobalContextMap.repr Σg')).
+  2:now depelim wf.
+  set (Σg := {| GlobalContextMap.global_decls := _ :: _ |}).
+  symmetry. eapply (optimize_env_extends' (Σ := Σg') (Σ' := Σg)) => //.
+  cbn. now exists [a].
+Qed.
+
+Lemma optimize_env_expanded {efl : EEnvFlags} {Σ : GlobalContextMap.t} :
+  wf_glob Σ -> expanded_global_env Σ -> expanded_global_env (optimize_env Σ).
+Proof.
+  unfold expanded_global_env; move=> wfg.
+  rewrite optimize_env_eq //.
+  destruct Σ as [Σ map repr wf]. cbn in *.
+  clear map repr.
+  induction 1; cbn; constructor; auto.
+  cbn in IHexpanded_global_declarations.
+  unshelve eapply IHexpanded_global_declarations. now depelim wfg. cbn. 
+  set (Σ' := GlobalContextMap.make _ _).
+  rewrite -(optimize_env_eq Σ'). cbn. now depelim wfg.
+  eapply (optimize_expanded_decl_irrel (Σ := Σ')). now depelim wfg.
+  now unshelve eapply (optimize_expanded_decl (Σ:=Σ')).
+Qed.
+
+Lemma optimize_wellformed {efl : EEnvFlags} {Σ : GlobalContextMap.t} n t :
   has_tBox -> has_tRel ->
   wf_glob Σ -> EWellformed.wellformed Σ n t -> EWellformed.wellformed Σ n (optimize Σ t).
 Proof.
   intros wfΣ hbox hrel.
   induction t in n |- * using EInduction.term_forall_list_ind => //.
   all:try solve [cbn; rtoProp; intuition auto; solve_all].
-  - cbn -[lookup_inductive]. move/and3P => [] hasc /andP[]hs ht hbrs.
-    destruct EGlobalEnv.inductive_isprop_and_pars as [[[|] _]|] => /= //.
+  - cbn -[GlobalContextMap.inductive_isprop_and_pars lookup_inductive]. move/and3P => [] hasc /andP[]hs ht hbrs.
+    destruct GlobalContextMap.inductive_isprop_and_pars as [[[|] _]|] => /= //.
     destruct l as [|[br n'] [|l']] eqn:eql; simpl.
     all:rewrite ?hasc ?hs /= ?andb_true_r.
     rewrite IHt //.
@@ -746,8 +811,8 @@ Proof.
     do 2 depelim X. solve_all.
     rtoProp; solve_all. solve_all.
     rtoProp; solve_all. solve_all.
-  - cbn -[lookup_inductive]. move/andP => [] /andP[]hasc hs ht.
-    destruct EGlobalEnv.inductive_isprop_and_pars as [[[|] _]|] => /= //.
+  - cbn -[GlobalContextMap.inductive_isprop_and_pars lookup_inductive]. move/andP => [] /andP[]hasc hs ht.
+    destruct GlobalContextMap.inductive_isprop_and_pars as [[[|] _]|] => /= //.
     all:rewrite hasc hs /=; eauto.
   - cbn. rtoProp; intuition auto; solve_all.
     unfold test_def in *. len. eauto.
@@ -757,7 +822,7 @@ Qed.
 
 Import EWellformed.
 
-Lemma optimize_wellformed_irrel {efl : EEnvFlags} Σ t :
+Lemma optimize_wellformed_irrel {efl : EEnvFlags} {Σ : GlobalContextMap.t} t :
   wf_glob Σ ->
   forall n, wellformed Σ n t -> wellformed (optimize_env Σ) n t.
 Proof.
@@ -784,7 +849,7 @@ Proof.
 Qed.
 
 
-Lemma optimize_wellformed_decl_irrel {efl : EEnvFlags} Σ d :
+Lemma optimize_wellformed_decl_irrel {efl : EEnvFlags} {Σ : GlobalContextMap.t} d :
   wf_glob Σ ->
   wf_global_decl Σ d -> wf_global_decl (optimize_env Σ) d.
 Proof.
@@ -793,7 +858,7 @@ Proof.
   now eapply optimize_wellformed_irrel.
 Qed.
 
-Lemma optimize_decl_wf {efl : EEnvFlags} Σ :
+Lemma optimize_decl_wf {efl : EEnvFlags} {Σ : GlobalContextMap.t} :
   has_tBox -> has_tRel -> wf_glob Σ -> 
   forall d, wf_global_decl Σ d -> wf_global_decl (optimize_env Σ) (optimize_decl Σ d).
 Proof.
@@ -806,39 +871,46 @@ Proof.
   now eapply optimize_wellformed => //.
 Qed.
 
-Lemma fresh_global_optimize_env Σ kn : 
+Lemma fresh_global_optimize_env {Σ : GlobalContextMap.t} kn : 
   fresh_global kn Σ ->
   fresh_global kn (optimize_env Σ).
 Proof.
-  induction 1; constructor; auto.
+  destruct Σ as [Σ map repr wf]; cbn in *.
+  induction 1; cbn; constructor; auto.
+  now eapply Forall_map; cbn.
 Qed.
 
-Lemma optimize_env_wf {efl : EEnvFlags} Σ :
+Lemma optimize_env_wf {efl : EEnvFlags} {Σ : GlobalContextMap.t} :
   has_tBox -> has_tRel -> 
   wf_glob Σ -> wf_glob (optimize_env Σ).
 Proof.
   intros hasb hasrel.
-  induction 1; cbn; constructor; auto.
-  - cbn. eapply optimize_decl_wf => //.
-  - cbn. now eapply fresh_global_optimize_env.
+  intros wfg. rewrite optimize_env_eq //.
+  destruct Σ as [Σ map repr wf]; cbn in *.
+  clear map repr.
+  induction wfg; cbn; constructor; auto.
+  - rewrite /= -(optimize_env_eq (GlobalContextMap.make Σ (fresh_globals_cons_inv wf))) //.
+    eapply optimize_decl_wf => //.
+  - rewrite /= -(optimize_env_eq (GlobalContextMap.make Σ (fresh_globals_cons_inv wf))) //.
+    now eapply fresh_global_optimize_env.
 Qed.
 
-Definition optimize_program (p : eprogram) :=
+Definition optimize_program (p : eprogram_env) :=
   (EOptimizePropDiscr.optimize_env p.1, EOptimizePropDiscr.optimize p.1 p.2).
 
-Definition optimize_program_wf {efl} (p : eprogram) {hastbox : has_tBox} {hastrel : has_tRel} :
-  wf_eprogram efl p -> wf_eprogram efl (optimize_program p).
+Definition optimize_program_wf {efl} (p : eprogram_env) {hastbox : has_tBox} {hastrel : has_tRel} :
+  wf_eprogram_env efl p -> wf_eprogram efl (optimize_program p).
 Proof.
   intros []; split.
   now eapply optimize_env_wf.
   cbn. eapply optimize_wellformed_irrel => //. now eapply optimize_wellformed.
 Qed.
 
-Definition optimize_program_expanded {efl} (p : eprogram) :
-  wf_eprogram efl p ->
-  expanded_eprogram_cstrs p -> expanded_eprogram_cstrs (optimize_program p).
+Definition optimize_program_expanded {efl} (p : eprogram_env) :
+  wf_eprogram_env efl p ->
+  expanded_eprogram_env_cstrs p -> expanded_eprogram_cstrs (optimize_program p).
 Proof.
-  unfold expanded_eprogram.
+  unfold expanded_eprogram_env_cstrs.
   move=> [wfe wft] /andP[] etae etat.
   apply/andP; split.
   cbn. eapply expanded_global_env_isEtaExp_env, optimize_env_expanded => //.
